\section{Fourier Analysis}
\subsection{CTFS}
\begin{align*}
    x(t) &= \sum_{n=-\infty}^\infty c_n e^{j2\pi nf_0 t}, c_n\in\mathbb{C}\\
    c_n &= \frac{1}{T_0}\int_{-\frac{T_0}{2}}^{\frac{T_0}{2}} x(t)e^{-j2\pi nf_0 t}dt\\
    P &= \sum_{n=-\infty}^\infty |c_n|^2 = \frac{1}{T_0}\int_{-\frac{T_0}{2}}^{\frac{T_0}{2}} |x(t)|^2 dt\\
    \intertext{Frequency response:}
    y(t) &= \sum_{k=1}^K c'_{k}e^{j(\omega_kt+\theta_k)}\\
    c'_k &= c_k\mathcal{H}(\omega_k)\\
    x(t) &= \sum_{k=1}^Kc_ke^{j(w_kt+\theta_k)}\\
    \mathcal{H}(\omega) &= \int_{-\infty}^\infty e^{-j\omega\tau}h(\tau)d\tau
\end{align*}
\subsection{CTFT}
\begin{align*}
    X(f) &= \int_{-\infty}^\infty x(t)e^{-j2\pi ft}dt\\
    x(t) &= \frac{1}{2\pi}\int_{-\infty}^\infty X(f) e^{j2\pi ft}dt\\
    &= \frac{1}{2\pi}\int_{-\infty}^\infty X(w) e^{jwt}dw\\
    E &= \int_{-\infty}^\infty |x(t)|^2dt = \int_{-\infty}^\infty |X(f)|^2df\\
    P &= \lim_{T\rightarrow \infty}\frac{1}{T}\int_{-T/2}^{T/2}|x(t)|^2 dt\\
    &= \int_{-\infty}^\infty S_{x_p}(f)df\\
    S_{x_p}(f) &= \sum_{n=-\infty}^\infty |c_n|^2\delta(f-nf_0)
\end{align*}
Properties
\begin{align*}
    a x_1(t) + b x_2(t) & \xleftrightarrow{\mathcal{F}} a X_1(f) + b X_2(f)\\
    x(a t) &\xleftrightarrow{\mathcal{F}} \frac{1}{|a|} X(\frac{f}{a})\\
    X(t) &\xleftrightarrow{\mathcal{F}} x(-f)\\
    x(t-t_1) &\xleftrightarrow{\mathcal{F}} e^{-j2\pi ft_1}X(f)\\
    e^{j2\pi f_1 t}x(t) &\xleftrightarrow{\mathcal{F}} X(f-f_1)\\
    \frac{d}{dt}x(t) &\xleftrightarrow{\mathcal{F}} j2\pi fX(f)\\
    \frac{d^n}{dt^n}x(t) &\xleftrightarrow{\mathcal{F}} (j2\pi f)^n X(f)\\
    \int_{-\infty}^t x(\tau)d\tau &\xleftrightarrow{\mathcal{F}} \frac{1}{j2\pi f}X(f) + \frac{1}{2}X(0)\delta(f)\\
    x_1(t) * x_2(t) &= \int_{-\infty}^\infty x_1(\tau)x_2(t-\tau)d\tau \xleftrightarrow{\mathcal{F}} X_1(f)X_2(f)\\
    x_1(t) x_2(t) &\xleftrightarrow{\mathcal{F}} \int_{\infty}^\infty X_1(\lambda)X_2(f-\lambda)d\lambda = X_1(f)*X_2(f)
\end{align*}
\subsection{DTFS}
\begin{align*}
    \intertext{Analysis}
    X(\Omega) &= \sum_{k=0}^{N-1}2\pi c_k \delta(\Omega-\frac{2\pi}{N}k)\\
    c_k &= \frac{1}{N}\sum_{n=0}^{N-1}\Tilde{x}[n]e^{-j\frac{2\pi}{N}\Omega kn}\\
    \intertext{Synthesis}
    \Tilde{x}[n] &= \sum_{k=0}^{N-1} c_k e^{j\frac{2\pi}{N}kn}, n\in \mathbb{Z}\\
    \Tilde{x}[n] &= \frac{1}{2T}\int_0^{2\pi}X(\Omega)e^{j\Omega n}d\Omega
\end{align*}
\subsection{DTFT}
\begin{align*}
    X(\Omega) &= \sum_{n=-\infty}^\infty x[n] e^{-j\Omega_n n}\\
    x[n] &= \frac{1}{2T}\int_0^{2\pi}X(\Omega)e^{j\Omega n}d\Omega
\end{align*}
\subsection{DFT}
\begin{align*}
    X[k] &= \sum_{n=0}^{N-1}x[n]e^{-j\frac{2\pi}{N}kn}\\
    x[n] &= \frac{1}{N}\sum_{k=0}^{N-1}X[k]e^{j\frac{2\pi}{N}kn}
\end{align*}
\subsection{Fourier Transform Pairs}
\begin{align*}
    \delta(t) &\xleftrightarrow{\mathcal{F}} 1\\
    \delta(t-t_0)f(t) &\xleftrightarrow{\mathcal{F}} e^{-j2\pi ft_0}f(t_0)\\
    e^{jw_0t} &\xleftrightarrow{\mathcal{F}} 2\pi \delta(w-w_0)\\
    e^{-at}u(t) &\xleftrightarrow{\mathcal{F}} \frac{1}{a + jw}\\
    \tri \frac{t}{T} &\xleftrightarrow{\mathcal{F}} T\sinc^2 (fT) = AT\frac{\sin (\pi ft)}{\pi ft}\\
    \cos (2\pi f_c t) &\xleftrightarrow{\mathcal{F}} \frac{1}{2}[\delta(f-f_0) + \delta(f + f_0)]\\
    \sin (2\pi f_c t) &\xleftrightarrow{\mathcal{F}} \frac{1}{2j}[\delta(f-f_0) - \delta(f + f_0)]
\end{align*}